src/Language/PlutusIR/Semantics/Misc/Axiom.v
@@ -5,9 +5,9 @@ Require Export PlutusCert.Language.PlutusIR.Analysis.BoundVars.
 Require Export PlutusCert.Language.PlutusIR.Analysis.UniqueBinders.
 Require Import PlutusCert.Language.PlutusIR.Semantics.Static.
 
-Axiom uniqueness : forall t, Term.unique t.
+Axiom uniqueness : forall t, unique_tm t.
 
 Axiom uniqueness' : forall (Delta : Delta) e,
   forall X,
-    Annotation.appears_bound_in X e ->
+    appears_bound_in_ann X e ->
     Delta X = None.
