src/Language/PlutusIR/Transform/FloatLet.v
@@ -265,7 +265,7 @@ Inductive transitive_closure (R : Term -> Term -> Prop) : Term -> Term -> Prop :
 
 
 Definition let_float t_pre t_post
-  := Term.unique t_pre
+  := unique_tm t_pre
   /\ well_typed t_post
   /\ exists t' t'',
     (  transitive_closure let_float_step t_pre t'
